# VE216 Lecture 17

>   Discrete Time Frequency Representations

## Complex Geometric Sequences

For the DT LTI $h[n]$ with input $x[n] = z^n$, we get $\begin{align}y[n] = (h*x)[n] = \sum^\infty_{k=-\infty} h[k]z^{n-k} = z^n\sum^\infty_{k=-\infty}h[k]z^{-k} = z^nH(z)\end{align}$

So $\begin{align}H(z) = \sum^\infty_{k=-\infty}h[k]z^{-k}\end{align}$, this is for DT Transform.

Remember CT Transform $\begin{align}H(s) = \int^\infty_{-\infty} h(t)e^{-st}dt\end{align}$

## Rational System Functions

We can derive $\sum z^{-k} Y = \sum z^{-p} Z$, then we can derive the $H(z) X = Y$ here.

## DT Vector Diagram

$\begin{align} H(z_0) = K\frac{\sum^{k_q}_{k=0} (z_0 - q_k)}{\sum^{r_p}_{r=0}(z_0 - p_r)} \end{align}$, very similar to CT Vector diagrams.

$\begin{align} |H(z_0)| = |K| \frac{\sum^{k_q}_{k=0} |z_0 - q_k|}{\sum^{r_p}_{r=0}|z_0 - p_r|}  \end{align}$ and $\angle H(z_0) = \angle K + \sum^{k_q}_{k=0} \angle (z_0-q_k) -  \sum^{r_p}_{r=0} \angle(z_0 - p_r)$.

## DT Frequency Response

$\begin{align}x[n] = \frac 1 2 (e^{j\Omega_0 n} + e^{-j\Omega_0 n}) \leftrightarrow y [n] &= \frac 1 2(H(e^{j\Omega_0}) e^{j\Omega_0 n} + H(e^{-j\Omega_0}) e^{-j\Omega_0 n} )\\&=\text{Re}\{H(e^{j\Omega_0}) e^{j\Omega_0 n} \}\\&=\text{Re}\{|H(e^{j\Omega_0}) |e^{j\angle H(e^{j\Omega_0})}e^{j\Omega_0 n} \}\\&=|H(e^{j\Omega_0})|\text{cos}(\Omega_0 n + \angle H(e^{j\Omega_0}))\end{align}$

### CT DT Frequency Responses Difference

-   CT Frequency Response: $H(s)$ on imaginary axis, $s = j\omega$
-   DT Frequency Response: $H(z)$ on unit circle, $z = e^{j\Omega}$

## DT Periodicity

Since $e^{j\Omega_2} = e^{j(\Omega_1 + 2\pi k)} = e^{j\Omega_1}$, then the "highest" DT frequency $\Omega = \pi$

<div style="page-break-after: always;"></div>

##  DT Fourier Series

$\begin{align} x[n] = x[n + N] = \sum^{N-1}_{k=0} a_k e^{kj\Omega_0n} \end{align}$ with $\Omega_0 = \frac {2\pi}N$

## Orthogonality

$\begin{align} \sum^{N-1}_{n=0} e^{j\Omega_0 kn}e^{-j\Omega_0ln} =  \sum^{N-1}_{n=0} e^{j\Omega_0 (k-l)n} = \begin{cases} N &k=l\\0 &k\neq l \end{cases} = N \delta[k-l] \end{align}$

So we get $\begin{align} a_k = \frac 1 N \sum^{N-1}_{n=0}x[n]e^{-jk\Omega_0 n} \end{align}$

-   Analysis equation: $\begin{align} a_k = a_{k+N} = \frac 1 N \sum_{n=<N>}x[n]e^{-jk\Omega_0 n} \end{align}$ $\Omega_0 = \frac {2\pi}N$
-   Synthesis equation: $\begin{align}x[n] = x[n+N] =\sum_{n=<N>}a_k e^{jk\Omega_0 n} \end{align}$

